DynamoDbEncryption/dafny/DynamoDbEncryptionTransforms/src/DynamoDbMiddlewareSupport.dfy
@@ -9,7 +9,7 @@
 include "DdbMiddlewareConfig.dfy"
 include "../../DynamoDbEncryption/src/DDBSupport.dfy"
 
-module DynamoDbMiddlewareSupport { 
+module DynamoDbMiddlewareSupport {
 
   import DDB = ComAmazonawsDynamodbTypes
   import opened AwsCryptographyDynamoDbEncryptionTransformsTypes
@@ -61,12 +61,15 @@ module DynamoDbMiddlewareSupport {
 
   // AddBeacons examines an AttributeMap and modifies it to be appropriate for Searchable Encryption,
   // returning a replacement AttributeMap.
-  function method {:opaque} AddBeacons(config : ValidTableConfig, item : DDB.AttributeMap)
-    : Result<DDB.AttributeMap, Error>
+  method AddBeacons(config : ValidTableConfig, item : DDB.AttributeMap)
+    returns (output : Result<DDB.AttributeMap, Error>)
     requires AwsCryptographyDynamoDbEncryptionItemEncryptorOperations.ValidInternalConfig?(config.itemEncryptor.config)
+    requires OneSearchValidState(config)
+    ensures OneSearchValidState(config)
+    modifies OneSearchModifies(config)
   {
-    BS.AddBeacons(config.search, item)
-      .MapFailure(e => E(e))
+    var ret := BS.AddBeacons(config.search, item);
+    return ret.MapFailure(e => AwsCryptographyDynamoDbEncryption(e));
   }
 
   // RemoveBeacons examines an AttributeMap and modifies it to be appropriate for customer use,
@@ -103,40 +106,50 @@ module DynamoDbMiddlewareSupport {
   }
 
   // Transform a QueryInput object for searchable encryption.
-  function method {:opaque} QueryInputForBeacons(config : ValidTableConfig, req : DDB.QueryInput)
-    : Result<DDB.QueryInput, Error>
+  method {:opaque} QueryInputForBeacons(config : ValidTableConfig, req : DDB.QueryInput)
+    returns (output : Result<DDB.QueryInput, Error>)
+    requires OneSearchValidState(config)
+    ensures OneSearchValidState(config)
+    modifies OneSearchModifies(config)
   {
-    BS.QueryInputForBeacons(config.search, req)
-      .MapFailure(e => AwsCryptographyDynamoDbEncryption(e))
+    var ret := BS.QueryInputForBeacons(config.search, req);
+    return ret.MapFailure(e => AwsCryptographyDynamoDbEncryption(e));
   }
 
   // Transform a QueryOutput object for searchable encryption.
-  function method {:opaque} QueryOutputForBeacons(config : ValidTableConfig, req : DDB.QueryInput, resp : DDB.QueryOutput)
-    : (ret : Result<DDB.QueryOutput, Error>)
+  method QueryOutputForBeacons(config : ValidTableConfig, req : DDB.QueryInput, resp : DDB.QueryOutput)
+    returns (output : Result<DDB.QueryOutput, Error>)
     requires resp.Items.Some?
-    ensures ret.Success? ==>
-      && ret.value.Items.Some?
+    ensures output.Success? ==> output.value.Items.Some?
+    requires OneSearchValidState(config)
+    ensures OneSearchValidState(config)
+    modifies OneSearchModifies(config)
   {
-    BS.QueryOutputForBeacons(config.search, req, resp)
-      .MapFailure(e => AwsCryptographyDynamoDbEncryption(e))
+    var ret := BS.QueryOutputForBeacons(config.search, req, resp);
+    return ret.MapFailure(e => AwsCryptographyDynamoDbEncryption(e));
   }
 
   // Transform a ScanInput object for searchable encryption.
-  function method {:opaque} ScanInputForBeacons(config : ValidTableConfig, req : DDB.ScanInput)
-    : Result<DDB.ScanInput, Error>
+  method ScanInputForBeacons(config : ValidTableConfig, req : DDB.ScanInput)
+    returns (output : Result<DDB.ScanInput, Error>)
+    requires OneSearchValidState(config)
+    ensures OneSearchValidState(config)
+    modifies OneSearchModifies(config)
   {
-    BS.ScanInputForBeacons(config.search, req)
-      .MapFailure(e => AwsCryptographyDynamoDbEncryption(e))
+    var ret := BS.ScanInputForBeacons(config.search, req);
+    return ret.MapFailure(e => AwsCryptographyDynamoDbEncryption(e));
   }
 
   // Transform a ScanOutput object for searchable encryption.
-  function method {:opaque} ScanOutputForBeacons(config : ValidTableConfig, req : DDB.ScanInput, resp : DDB.ScanOutput)
-    : (ret : Result<DDB.ScanOutput, Error>)
+  method ScanOutputForBeacons(config : ValidTableConfig, req : DDB.ScanInput, resp : DDB.ScanOutput)
+    returns (output : Result<DDB.ScanOutput, Error>)
     requires resp.Items.Some?
-    ensures ret.Success? ==>
-      && ret.value.Items.Some?
+    ensures output.Success? ==> output.value.Items.Some?
+    requires OneSearchValidState(config)
+    ensures OneSearchValidState(config)
+    modifies OneSearchModifies(config)
   {
-    BS.ScanOutputForBeacons(config.search, req, resp)
-      .MapFailure(e => AwsCryptographyDynamoDbEncryption(e))
+    var ret := BS.ScanOutputForBeacons(config.search, req, resp);
+    return ret.MapFailure(e => AwsCryptographyDynamoDbEncryption(e));
   }
 }
