DynamoDbEncryption/dafny/DynamoDbEncryptionTransforms/test/BatchExecuteStatementTransform.dfy
@@ -12,14 +12,15 @@ module BatchExecuteStatementTransformTest {
 
   method {:test} TestBatchExecuteStatementInputPassthrough() {
     var middlewareUnderTest := TestFixtures.GetDynamoDbEncryptionTransforms();
+    var statement := GetStatement("update \"no_such_table\"");
+    var request := DDB.BatchStatementRequest(
+      Statement := statement,
+      Parameters := None(),
+      ConsistentRead := None()
+    );
+    var requests := GetPartiQLBatchRequest([request]);
     var good_input := DDB.BatchExecuteStatementInput(
-      Statements := [
-        DDB.BatchStatementRequest(
-          Statement := "update \"no_such_table\"",
-          Parameters := None(),
-          ConsistentRead := None()
-        )
-      ],
+      Statements := requests,
       ReturnConsumedCapacity := None()
     );
     var good_transformed := middlewareUnderTest.BatchExecuteStatementInputTransform(
@@ -34,14 +35,15 @@ module BatchExecuteStatementTransformTest {
 
   method {:test} TestBatchExecuteStatementInputEncrypted() {
     var middlewareUnderTest := TestFixtures.GetDynamoDbEncryptionTransforms();
+    var statement := GetStatement("update \"foo\"");
+    var request := DDB.BatchStatementRequest(
+      Statement := statement,
+      Parameters := None(),
+      ConsistentRead := None()
+    );
+    var requests := GetPartiQLBatchRequest([request]);
     var bad_input := DDB.BatchExecuteStatementInput(
-      Statements := [
-        DDB.BatchStatementRequest(
-          Statement := "update \"foo\"",
-          Parameters := None(),
-          ConsistentRead := None()
-        )
-      ],
+      Statements := requests,
       ReturnConsumedCapacity := None()
     );
     var bad_transformed := middlewareUnderTest.BatchExecuteStatementInputTransform(
@@ -61,6 +63,7 @@ module BatchExecuteStatementTransformTest {
       Responses := None(),
       ConsumedCapacity := None()
     );
+    var statement := GetStatement("foo");
     var input := DDB.BatchExecuteStatementInput(
       Statements := [
         DDB.BatchStatementRequest(
